simulation

Cslib/Semantics/LTS/Simulation.lean
@@ -1,4 +1,120 @@
-import Cslib.Semantics.LTS.Basic
+/-
+Copyright (c) 2025 Fabrizio Montesi. All rights reserved.
+Released under Apache 2.0 license as described in the file LICENSE.
+Authors: Fabrizio Montesi
+-/
 
+import Cslib.Semantics.LTS.Basic
+import Cslib.Utils.Rel
+
+/-! # Simulation and Similarity
+
+A simulation is a binary relation on the states of an `LTS`: if two states `s1` and `s2` are related by a simulation, then
+`s2` can mimic all transitions of `s1`. Furthermore, the derivatives reaches through
+these transitions remain related by the simulation.
+
+Similarity is the largest simulation: given an `LTS`, it relates any two states that are related
+by a bisimulation for that LTS.
+
+For an introduction to theory of simulation, we refer to [Sangiorgi2011].
+
+## Main definitions
+
+- `Simulation lts r`: the relation `r` on the states of the LTS `lts` is a simulation.
+- `Similarity lts` is the binary relation on the states of `lts` that relates any two states
+related by some simulation on `lts`.
+- `SimulationEquiv lts` is the binary relation on the states of `lts` that relates any two states
+similar to each other.
+
+## Notations
+
+- `s1 ≤[lts] s2`: the states `s1` and `s2` are similar in the LTS `lts`.
+- `s1 ≤[lts]≥ s2`: the states `s1` and `s2` are simulation equivalent in the LTS `lts`.
+
+## Main statements
+
+## TODOs
+
+- `SimulationEquiv.eqv`: simulation equivalence is an equivalence relation (see `Equivalence`).
+- Connections between similarity, simulation equivalence, bisimilarity, and trace equivalence.
+
+-/
+
+universe u v
+
+section Simulation
+
+variable {State : Type u} {Label : Type v} (lts : LTS State Label)
+
+/-- A relation is a simulation if, whenever it relates two states in an lts,
+any transition originating from the first state is mimicked by a transition from the second state
+and the reached derivatives are themselves related. -/
 def Simulation (lts : LTS State Label) (r : Rel State State) : Prop :=
   ∀ s1 s2, r s1 s2 → ∀ μ s1', lts.tr s1 μ s1' → ∃ s2', lts.tr s2 μ s2' ∧ r s1' s2'
+
+/-- Two states are similar if they are related by some simulation. -/
+def Similarity (lts : LTS State Label) : Rel State State :=
+  fun s1 s2 =>
+    ∃ r : Rel State State, r s1 s2 ∧ Simulation lts r
+
+/--
+Notation for similarity.
+
+Differently from standard pen-and-paper presentations, we require the lts to be mentioned
+explicitly.
+-/
+notation s:max " ≤[" lts "] " s':max => Similarity lts s s'
+
+/-- Similarity is reflexive. -/
+theorem Similarity.refl (s : State) : s ≤[lts] s := by
+  exists Rel.Id
+  apply And.intro (by constructor)
+  simp only [Simulation]
+  intro s1 s2 hr μ s1' htr
+  cases hr
+  exists s1'
+  apply And.intro htr (by constructor)
+
+/-- The composition of two simulations is a simulation. -/
+theorem Simulation.comp
+  (r1 r2 : Rel State State) (h1 : Simulation lts r1) (h2 : Simulation lts r2) :
+  Simulation lts (r1.comp r2) := by
+  simp_all only [Simulation]
+  intro s1 s2 hrc μ s1' htr
+  rcases hrc with ⟨sb, hr1, hr2⟩
+  specialize h1 s1 sb hr1 μ
+  specialize h2 sb s2 hr2 μ
+  have h1' := h1 s1' htr
+  obtain ⟨s1'', h1'tr, h1'⟩ := h1'
+  have h2' := h2 s1'' h1'tr
+  obtain ⟨s2'', h2'tr, h2'⟩ := h2'
+  exists s2''
+  constructor
+  · exact h2'tr
+  · simp [Rel.comp]
+    exists s1''
+
+/-- Similarity is transitive. -/
+theorem Similarity.trans (h1 : s1 ≤[lts] s2) (h2 : s2 ≤[lts] s3) : s1 ≤[lts] s3 := by
+  obtain ⟨r1, hr1, hr1s⟩ := h1
+  obtain ⟨r2, hr2, hr2s⟩ := h2
+  exists r1.comp r2
+  constructor
+  case left =>
+    simp only [Rel.comp]
+    exists s2
+  case right =>
+    apply Simulation.comp lts r1 r2 hr1s hr2s
+
+/-- Simulation equivalence relates all states `s1` and `s2` such that `s1 ≤[lts] s2` and
+`s2 ≤[lts] s1`. -/
+def SimulationEquiv (lts : LTS State Label) : Rel State State :=
+  fun s1 s2 =>
+    s1 ≤[lts] s2 ∧ s2 ≤[lts] s1
+
+/--
+Notation for simulation equivalence.
+-/
+notation s:max " ≤[" lts "]≥ " s':max => SimulationEquiv lts s s'
+
+end Simulation
